Add triples for reading from disk0
There are two different rules, based on whether one has the knowledge that
disk1 has failed (in which case, we can guarantee that the read from disk0 will
fail).

src/Examples/ReplicatedDisk/WeakestPre.v
@@ -444,10 +444,17 @@ Ltac inv_step :=
          | [ H : such_that _ _ _ |- _ ] => inversion H; subst; clear H
          | [ H : pure _ _ _ |- _ ] => inversion H; subst; clear H
          | [ H: puts _ _ _ |- _ ] => inversion H; subst; clear H
+         | [ H: reads _ _ _ |- _ ] => inversion H; subst; clear H
          | [ H : Some _ = Some _ |- _] => apply Some_inj in H; subst
          | [ H : Cinl _ = Cinl _ |- _] => inversion H; clear H; subst
          | [ H : (?a, ?b) = (?c, ?d) |- _] => apply pair_inj in H as (?&?); subst
          | [ H : disk_fail _ Err |- _] => exfalso; eapply disk_fail_non_err; eauto
+         | [ H: l.(Layer.sem).(Proc.step) ?op _ (Val _ _) |- _] =>
+           let Hhd := fresh "Hhd" in
+           let Htl := fresh "Htl" in
+           destruct H as (?&?&Hhd&Htl)
+         | [ H: l.(Layer.sem).(Proc.step) ?op _ (Val _ _) |- _] =>
+           inversion H; subst
          end; auto with twodb).
 
     Ltac inv_case :=
@@ -478,8 +485,7 @@ Proof.
   }
   iIntros (e2 (n2, σ2) Hstep) "!>".
   inversion Hstep; subst.
-  inversion H0 as ([]&?&Hhd&Htl).
-  inversion Htl; subst.
+  inv_step.
   iDestruct "Hown" as "(?&Hown)".
   iDestruct "Hown" as (mems disk0 disk1) "(Hmem&Hown0&Hown1&Hstatus&Hp)".
   iDestruct "Hp" as %(Heq_mem&Heq_disk&?&Hsize).
@@ -495,7 +501,7 @@ Proof.
     { iPureIntro.
       split_and!; eauto; inv_step .
       rewrite Heq_state => //=.
-      destruct x => //=.
+      destruct x0 => //=.
       simpl in *. subst. simpl; intuition; eauto.
       rewrite /upd_default.
       * rewrite /upd_disk/upd_default Hin_bound //.
@@ -523,7 +529,7 @@ Proof.
       iPureIntro.
       split_and!; eauto.
       ** rewrite /upd_disk/upd_default Heq_state => //=.
-         destruct x => //=.
+         destruct x0 => //=.
          simpl in *. subst. simpl; intuition; eauto.
          rewrite Hin_bound //.
       ** split_and!; intuition eauto with twodb.
@@ -536,33 +542,137 @@ Proof.
       iPureIntro.
       split_and!; eauto.
       ** rewrite /upd_disk/upd_default Heq_state => //=.
-         destruct x => //=.
+         destruct x0 => //=.
          simpl in *. subst. simpl; intuition; eauto.
       ** split_and!; intuition eauto with twodb.
   }
   by iApply "HΦ".
 Qed.
 
-(*
-Lemma wp_read_disk s E i v :
-  {{{ ▷ i d↦ v }}} read_disk i @ s; E {{{ RET v; i d↦ v }}}.
+Definition status_token (ds: DisksState) : iProp Σ :=
+  match ds with
+    | BothDisks _ _ => True%I
+    | OnlyDisk id _ => is_OnlyDisk id
+  end.
+
+Lemma disk_status_update σ σ' u:
+  disk_fail σ (Val σ' u) →
+  disk_status_ctx σ.(disks_state) ==∗
+  (disk_status_ctx σ'.(disks_state) ∗ status_token σ'.(disks_state)).
+Proof.
+  intros Hfail.
+  destruct σ as (?&[]).
+  * inversion Hfail; inv_step; try inv_case; inv_step; eauto => //=;
+    iIntros "H"; eauto; iMod (disk_status_update_both with "[$]") as "H"; eauto.
+  * eapply disk_fail_only_one in Hfail; subst; eauto.
+Qed.
+
+Lemma wp_read_disk0 s E i v :
+  {{{ ▷ i d0↦ v }}}
+    read_disk d0 i @ s; E
+  {{{ mv, RET mv;
+      i d0↦ v ∗ match mv with
+                | None => is_OnlyDisk d1
+                | Some v' => ⌜ v = v' ⌝
+                end }}}.
 Proof.
   iIntros (Φ) ">Hi HΦ". iApply wp_lift_call_step.
   iIntros ((n, σ)) "Hown".
-  iModIntro. iSplit; first by destruct s.
+  iModIntro. iSplit.
+  { destruct s; auto. iPureIntro. apply snd_lift_non_err.
+    inversion 1; inv_step. repeat deex. inv_step.
+  }
   iIntros (e2 (n2, σ2) Hstep) "!>".
   inversion Hstep; subst.
-  inversion H0; subst.
+  inv_step.
   iDestruct "Hown" as "(?&Hown)".
-  iDestruct "Hown" as (mems disks) "(Hown1&Hown2&Hp)".
+  iDestruct "Hown" as (mems disk0 disk1) "(Hown_mem&Hown0&Hown1&Hstatus&Hp)".
   iDestruct "Hp" as %(Heq_mem&Heq_disk&Hsize&?).
-  iDestruct (gen_heap_valid with "Hown2 Hi") as %Hin_bound.
-  iModIntro. iSplitR "Hi HΦ".
-  - iFrame. iExists _, _. iFrame; iPureIntro; split_and!; eauto.
-  - rewrite /get_disk/get_default -Heq_disk Hin_bound.
-    by iApply "HΦ".
+  iDestruct (gen_heap_valid with "Hown0 Hi") as %Hin_bound.
+  simpl in Heq_disk.
+  iMod (disk_status_update with "Hstatus") as "($&Htok)"; first eauto.
+  destruct (σ.(disks_state)) as [?|?] eqn:Heq_state.
+  - simpl. iFrame. iSplitR "Hi HΦ Htok".
+    * iExists _, disk0, disk1. iFrame.
+      iFrame. simpl. intuition; eauto. subst.
+      inversion Hhd.
+      { iPureIntro.
+        split_and!; eauto; inv_step .
+        rewrite Heq_state => //=.
+        split_and!; intuition eauto with twodb.
+      }
+      inv_case; inv_step.
+      { iPureIntro.
+        split_and!; eauto.
+        subst; rewrite /maybe_fail_disk Heq_state => //=.
+        split_and!; intuition eauto with twodb.
+      }
+      { iPureIntro.
+        split_and!; eauto.
+        subst; rewrite /maybe_fail_disk Heq_state => //=.
+        split_and!; intuition eauto with twodb.
+      }
+    * inversion Hhd.
+      {
+        rewrite /lookup_disk/get_disk/TwoDisk.disk0. inv_step. rewrite Heq_state.
+        rewrite /lookup_default. intuition. subst. rewrite Hin_bound.
+        iApply "HΦ"; eauto.
+      }
+      inv_case; inv_step.
+      {
+        rewrite /lookup_disk/get_disk/maybe_fail_disk Heq_state //=.
+        iApply "HΦ"; eauto.
+      }
+      {
+        rewrite /lookup_disk/get_disk/maybe_fail_disk Heq_state //=.
+        rewrite /lookup_default. intuition. subst. rewrite Hin_bound.
+        iApply "HΦ"; eauto.
+      }
+  - eapply disk_fail_only_one in Hhd; eauto. subst.
+    simpl. iFrame. iSplitR "Hi HΦ Htok".
+    * iExists _, disk0, disk1. iFrame.
+      iFrame. simpl. intuition; eauto. subst.
+      iPureIntro.
+      split_and!; eauto.
+      subst; rewrite /maybe_fail_disk Heq_state => //=.
+      split_and!; intuition eauto with twodb.
+    * rewrite /lookup_disk/get_disk/TwoDisk.disk0/TwoDisk.disk1 ?Heq_state //=.
+      destruct id; rewrite /lookup_default; intuition; subst; rewrite ?Hin_bound;
+      iApply "HΦ"; eauto.
 Qed.
-*)
+
+Lemma wp_read_disk0_only0 s E i v :
+  {{{ ▷ i d0↦ v ∗ ▷ is_OnlyDisk d0 }}}
+    read_disk d0 i @ s; E
+  {{{ RET (Some v); i d0↦ v }}}.
+Proof.
+  iIntros (Φ) "(>Hi&>His_only) HΦ". iApply wp_lift_call_step.
+  iIntros ((n, σ)) "Hown".
+  iModIntro. iSplit.
+  { destruct s; auto. iPureIntro. apply snd_lift_non_err.
+    inversion 1; inv_step. repeat deex. inv_step.
+  }
+  iIntros (e2 (n2, σ2) Hstep) "!>".
+  inversion Hstep; subst.
+  inv_step.
+  iDestruct "Hown" as "(?&Hown)".
+  iDestruct "Hown" as (mems disk0 disk1) "(Hown_mem&Hown0&Hown1&Hstatus&Hp)".
+  iDestruct "Hp" as %(Heq_mem&Heq_disk&Hsize&?).
+  iDestruct (gen_heap_valid with "Hown0 Hi") as %Hin_bound.
+  iDestruct (disk_status_agree with "[$] [$]") as %Hstatus.
+  destruct Hstatus as (disk0'&Heq). simpl in *.
+  rewrite Heq in Heq_disk. subst.
+  eapply disk_fail_only_one in Hhd; eauto. subst.
+  iFrame. iSplitR "Hi HΦ".
+    * iExists _, disk0', disk1. iFrame.
+      iPureIntro.
+      split_and!; eauto; inv_step.
+      rewrite Heq => //=.
+      split_and!; intuition eauto with twodb.
+    * rewrite /lookup_disk/get_disk/TwoDisk.disk0. inv_step. rewrite Heq.
+      rewrite /lookup_default. intuition. subst. rewrite Hin_bound.
+      iApply "HΦ"; eauto.
+Qed.
 
 End lifting.
 
